Remove unit

SSASlow.lean
@@ -1,22 +1,19 @@
-inductive Kind where
-| k_a : Kind
-
 inductive Op where
-| op (name : String) (argval : Unit)
+| op (name : String)
 
 def sem: (o: Op) → Unit
-| .op "a" _ => ()
-| .op "b" _ => ()
-| .op "c" _ => ()
-| .op "d" _ => ()
-| .op "e" _ => ()
-| .op "f" _ => ()
-| .op "g" _ => ()
-| .op "h" _ => ()
-| .op "i" _ => ()
+| .op "a" => ()
+| .op "b" => ()
+| .op "c" => ()
+| .op "d" => ()
+| .op "e" => ()
+| .op "f" => ()
+| .op "g" => ()
+| .op "h" => ()
+| .op "i" => ()
 | _ => ()
 
-theorem Fail: sem (.op "x" ()) = output  := by {
+theorem Fail: sem (.op "x") = output  := by {
   -- tactic 'simp' failed, nested error:
   -- (deterministic) timeout at 'whnf', maximum number of heartbeats (200000) has been reached (use 'set_option maxHeartbeats <num>' to set the limit)
   simp only[sem];
